theories/LAM/TM/LMBounds_Loop.v
@@ -5,9 +5,9 @@ From Undecidability Require Import LM_heap_def TM.PrettyBounds.MaxList.
 
 From Undecidability.LAM Require Import TM.Alphabets.
 From Undecidability.LAM.TM Require Import CaseCom.
-From Undecidability.LAM.TM Require Import StepTM LMBounds HaltingProblem.
+From Undecidability.LAM.TM Require Import StepTM LMBounds HaltingProblem SizeAnalysis.
 
-From Undecidability Require Import UpToCNary.
+From Undecidability Require Import UpToC UpToCNary.
 Print Loop_steps.
 Check LM.Step_steps_nice.
 
@@ -46,34 +46,141 @@ Proof.
   unfold sizeP;cbn. rewrite size_sizeT_le.
   specialize (sizeT_ge_1 t). nia.
 Qed.
-*)  
+ *)
+
+Lemma size_list (sig X : Type) (cX : codable sig X) (xs : list X):
+  size xs = length xs + sumn (map size xs) + 1.
+Proof.
+  induction xs. now rewrite encodeList_size_nil.
+  rewrite encodeList_size_cons. cbn [length map sumn]. nia.
+Qed.
+
+Lemma size_list_le_bound (sig X : Type) (cX : codable sig X) (xs : list X) c:
+  (forall x, x el xs -> size x <= c)
+  -> size xs <= length xs * (c+1) + 1.
+Proof.
+  intros H. rewrite size_list. rewrite sumn_le_bound.
+  2:{ intros ?. rewrite in_map_iff. intros (?&<-&?). eauto. }
+  rewrite map_length. nia.
+Qed.
+
+Lemma size_HClos_le (g : HClos):
+  size g = fst g + size (snd g) + 1.
+Proof.
+  rewrite Encode_Clos_hasSize. destruct g as [a P];cbn.
+  replace (Encode_list_size _ P) with (size P). nia. apply Encode_list_hasSize.
+Qed.
+
+Lemma heap_greatest_address2_bound H c:
+  (forall P a, Some (P,a) el H -> a <= c) -> LM_Lookup_nice.heap_greatest_address2 H <= c.
+Proof.
+  induction H as [ | [ [] | ] ]. all:cbn.
+  -easy.
+  -intros H'. rewrite IHlist. rewrite H' with (a:=n). all:now auto.
+  -eauto.
+Qed.
 
 Section FixInit.
+  Variable H__init: list HEntr.
 
-  Variable T V : list HClos.
+  (*Variable T V : list HClos.
   Variable H H__init: list HEntr.
   Variable i : nat.
-
-  Variable P0 : Pro.
-  Hypothesis R: pow step i ([(0,P0)],[],H__init) (T,V,H).
+  *)
+  (*Hypothesis R: pow step i ([(0,P0)],[],H__init) (T,V,H).*)
   Hypothesis empty_H__init: forall c, c el H__init -> c = None.
-  (*
-  Lemma Step_steps_nice :
+
+  Lemma Step_steps_nicer :
     {c : nat |
-      forall (T V : list HClos) (H : Heap),
+      forall P0 (T V : list HClos) (H : Heap) i,
         pow step i ([(0,P0)],[],H__init) (T,V,H)
-        -> Step_steps T V H <=(c) (let a := length H__init + i in
-                                 1 + a + 
-                                size a + size H + size V +
-                                size P * (1 + size H + Init.Nat.max a (LM_Lookup_nice.heap_greatest_address2 H) + size P)
-                              end}.
+        -> Step_steps T V H <=(c) (length H__init + i +1 + sizeP P0 )^3}.
+  Proof.
+    eexists. intros P0 T V H i H0. eapply dominatedWith_trans. eapply (proj2_sig LM.Step_steps_nice).
+    destruct T as [ | [a P] T].
+    2:{
+      set (lH := length H__init + i). cbn zeta.
+      specialize SizeAnalysis.size_clos with (1:=H0) (2:=empty_H__init)as Hsize.
+      repeat setoid_rewrite size_le_sizeP. rewrite !Encode_nat_hasSize.
+      erewrite size_list_le_bound with (xs:=V).
+      2:{ intros [a' P'] ?. rewrite size_HClos_le. cbn.
+          rewrite size_le_sizeP.
+          edestruct (Hsize P' a') as [[-> ->] _]. now eauto. reflexivity.
+      }
+      unfold Encode_Heap, sigHeap. erewrite size_list_le_bound with (xs:=H).
+      2:{ intros [[[a' P'] beta] | ] ?. 2:cbv.  
+          -apply Hsize in H1. unfold sigHEntr,HEntr,Encode_HEntr,sigHEntr',Encode_HEntr'. rewrite Encode_option_hasSize.
+           cbn. rewrite Encode_pair_hasSize;cbn. rewrite size_HClos_le. cbn.
+           rewrite size_le_sizeP, Encode_nat_hasSize. destruct H1 as (->&->&->). reflexivity.
+          -nia. 
+      }
+      rewrite heap_greatest_address2_bound.
+      2:{ intros [] ?. edestruct Hsize as [_ H']. apply H'. }
+      specialize Hsize with (P1:=P) (a0 := a) as [(-> & -> ) _]. easy.
+      rewrite Nat.max_id.
+      specialize length_TV  with (1:=H0) (2:=empty_H__init) as H_TV. cbn in H_TV.
+      assert (length V <= i) as -> by nia.
+      specialize length_H  with (1:=H0) (2:=empty_H__init) as ->. fold lH.
+      clear dependent T. clear dependent V. clear dependent H.  clear dependent P. clear dependent a.
+      assert (i<=lH) as -> by nia.
+      clearbody lH. clear dependent H__init.
+      cbn [Nat.pow].
+      ring_simplify. instantiate (1:=9). hnf. lia.
+    }
+    cbn. hnf. lia.
+  Qed.
 
-Lemma Loop_steps_nice' :
-  (fun '(T,V,H,k) => Loop_steps [c] [] [] k) <=c (fun '(T,V,H,k) => 1).
-Proof.
+  Lemma Loop_steps_nice' :
+    {c : nat |
+      forall P0 (T V : list HClos) (H : Heap) k i,
+       pow step i ([(0,P0)],[],H__init) (T,V,H)
+        -> Loop_steps T V H k <=(c) (k + 1) * (length H__init + (i+k) +1 + sizeP P0 )^3}.
+  Proof.
+    evar (c:nat).
+    eexists c. intros P0 T V H k.
+    induction k in T,V,H |-*.
+    all:intros i Hi.
+    all:cbn - [Step_steps Nat.pow step_fun plus].
+    -eapply dominatedWith_mono_c. eapply dominatedWith_trans. now apply (proj2_sig Step_steps_nicer). apply dominatedWith_solve. now cbn.
+     ring_simplify. shelve. 
+    -destruct (step_fun (T, V, H)) as [[[T' V'] H'] | ]  eqn:Hstep.
+     2:{ eapply dominatedWith_mono_c. eapply dominatedWith_trans. now apply (proj2_sig Step_steps_nicer). apply dominatedWith_solve. now cbn.
+         ring_simplify. shelve. }
+     destruct is_halt_state.
+     1:{ eapply dominatedWith_mono_c. all:repeat simple apply dominatedWith_add.
+         1: apply dominatedWith_solve; now cbn.
+         1,2: eapply dominatedWith_trans;[eapply (proj2_sig Step_steps_nicer) | ].
+         easy. 2:{eapply pow_add. eexists;split. easy. rewrite <- rcomp_1. now apply step_fun_step. }
+         1,2: apply dominatedWith_solve;now cbn. ring_simplify. shelve.
+     }
+     Set Nested Proofs Allowed.
+     Lemma dominatedWith_add_split (c x1 x2 y1 y2 : nat) :
+       x1 <=(c) y1 -> x2 <=(c) y2 -> x1 + x2 <=(c) y1 + y2.
+     Proof.
+       unfold dominatedWith. nia.
+     Qed.
+     set (tmp:= _ ^ 3). replace ( (S k + 1) * tmp) with (tmp + (k+1) * tmp) by nia.
+     apply dominatedWith_add_split;subst tmp.
+     { eapply dominatedWith_mono_c. eapply dominatedWith_add.
+       -apply dominatedWith_solve. now cbn.
+       -eapply dominatedWith_trans. now apply (proj2_sig Step_steps_nicer). apply dominatedWith_solve. now cbn.
+       -ring_simplify. shelve.
+     }
+     replace (i + S k) with (i+1+k) by nia.
+     eapply IHk.
+     eapply pow_add. eexists;split. easy. rewrite <- rcomp_1. now apply step_fun_step.
+     Unshelve.
+     [c]:exact (2 * proj1_sig Step_steps_nicer + 1). all:subst c;nia.
+  Qed.
 
-Lemma Loop_steps_nice :
-  (fun '(T,V,H,k) => Loop_steps [c] [] [] k) <=c (fun '(T,V,H,k) => 1).
-Proof.
-   *)
+  Lemma Loop_steps_nice :
+    (fun '(P0,k) => Loop_steps [(0,P0)] [] H__init k)
+    <=c (fun '(P0,k) => (k + 1) * (length H__init + k +1 + sizeP P0 )^3).
+  Proof.
+    eexists. intros [? ?].
+    assert (H':= proj2_sig Loop_steps_nice'). cbn beta in H'. unfold dominatedWith in H'. 
+    specialize H' with (i:=0). cbn [plus] in H'.
+    rewrite H'. 2:reflexivity. reflexivity.
+  Qed.
 End FixInit.
+
